src/Init/Data/Array/Erase.lean
@@ -6,9 +6,10 @@ Authors: Kim Morrison
 prelude
 import Init.Data.Array.Lemmas
 import Init.Data.List.Nat.Erase
+import Init.Data.List.Nat.Basic
 
 /-!
-# Lemmas about `Array.eraseP` and `Array.erase`.
+# Lemmas about `Array.eraseP`, `Array.erase`, and `Array.eraseIdx`.
 -/
 
 namespace Array
@@ -17,11 +18,17 @@ open Nat
 
 /-! ### eraseP -/
 
-@[simp] theorem eraseP_nil : #[].eraseP p = #[] := rfl
+@[simp] theorem eraseP_empty : #[].eraseP p = #[] := rfl
 
-theorem eraseP_of_forall_not {l : Array α} (h : ∀ a, a ∈ l → ¬p a) : l.eraseP p = l := by
+theorem eraseP_of_forall_mem_not {l : Array α} (h : ∀ a, a ∈ l → ¬p a) : l.eraseP p = l := by
   cases l
   simp_all [List.eraseP_of_forall_not]
+
+theorem eraseP_of_forall_getElem_not {l : Array α} (h : ∀ i, (h : i < l.size) → ¬p l[i]) : l.eraseP p = l :=
+  eraseP_of_forall_mem_not fun a m => by
+    rw [mem_iff_getElem] at m
+    obtain ⟨i, w, rfl⟩ := m
+    exact h i w
 
 @[simp] theorem eraseP_eq_empty_iff {xs : Array α} {p : α → Bool} : xs.eraseP p = #[] ↔ xs = #[] ∨ ∃ x, p x ∧ xs = #[x] := by
   cases xs
@@ -43,7 +50,7 @@ theorem exists_or_eq_self_of_eraseP (p) (l : Array α) :
     let ⟨_, ha, pa⟩ := h
     .inr (exists_of_eraseP ha pa)
   else
-    .inl (eraseP_of_forall_not (h ⟨·, ·, ·⟩))
+    .inl (eraseP_of_forall_mem_not (h ⟨·, ·, ·⟩))
 
 @[simp] theorem size_eraseP_of_mem {l : Array α} (al : a ∈ l) (pa : p a) :
     (l.eraseP p).size = l.size - 1 := by
@@ -56,9 +63,8 @@ theorem size_eraseP {l : Array α} : (l.eraseP p).size = if l.any p then l.size 
     obtain ⟨i, h, w⟩ := h
     simp [size_eraseP_of_mem (l := l) (by simp) w]
   · simp only [any_eq_true] at h
-    rw [eraseP_of_forall_not]
+    rw [eraseP_of_forall_getElem_not]
     simp_all
-    sorry
 
 theorem size_eraseP_le (l : Array α) : (l.eraseP p).size ≤ l.size := by
   rcases l with ⟨l⟩
@@ -135,7 +141,13 @@ theorem eraseP_eq_iff {p} {l : Array α} :
   rcases l with ⟨l⟩
   rcases l' with ⟨l'⟩
   simp [List.eraseP_eq_iff]
-  sorry
+  constructor
+  · rintro (h | ⟨a, l₁, h₁, h₂, ⟨x, rfl, rfl⟩⟩)
+    · exact Or.inl h
+    · exact Or.inr ⟨a, ⟨l₁⟩, by simpa using h₁, h₂, ⟨⟨x⟩, by simp⟩⟩
+  · rintro (h | ⟨a, ⟨l₁⟩, h₁, h₂, ⟨⟨x⟩, rfl, rfl⟩⟩)
+    · exact Or.inl h
+    · exact Or.inr ⟨a, l₁, by simpa using h₁, h₂, ⟨x, by simp⟩⟩
 
 theorem eraseP_comm {l : Array α} (h : ∀ a ∈ l, ¬ p a ∨ ¬ q a) :
     (l.eraseP p).eraseP q = (l.eraseP q).eraseP p := by
@@ -164,7 +176,7 @@ theorem erase_eq_eraseP [LawfulBEq α] (a : α) (l : Array α) : l.erase a = l.e
   rcases xs with ⟨xs⟩
   simp [List.erase_eq_nil_iff]
 
-theorem erase_ne_nil_iff [LawfulBEq α] {xs : Array α} {a : α} :
+theorem erase_ne_empty_iff [LawfulBEq α] {xs : Array α} {a : α} :
     xs.erase a ≠ #[] ↔ xs ≠ #[] ∧ xs ≠ #[a] := by
   rcases xs with ⟨xs⟩
   simp [List.erase_ne_nil_iff]
@@ -181,7 +193,8 @@ theorem exists_erase_eq [LawfulBEq α] {a : α} {l : Array α} (h : a ∈ l) :
 theorem size_erase [LawfulBEq α] (a : α) (l : Array α) :
     (l.erase a).size = if a ∈ l then l.size - 1 else l.size := by
   rw [erase_eq_eraseP, size_eraseP]
-  sorry
+  congr
+  simp [mem_iff_getElem, eq_comm (a := a)]
 
 theorem size_erase_le (a : α) (l : Array α) : (l.erase a).size ≤ l.size := by
   rcases l with ⟨l⟩
@@ -301,14 +314,14 @@ theorem getElem_eraseIdx (l : Array α) (i : Nat) (h : i < l.size) (j : Nat) (h'
   rw [← getElem?_eq_getElem, getElem?_eraseIdx]
   split <;> simp
 
-@[simp] theorem eraseIdx_eq_nil_iff {l : Array α} {i : Nat} {h} : eraseIdx l i = #[] ↔ l.size = 1 ∧ i = 0 := by
+@[simp] theorem eraseIdx_eq_empty_iff {l : Array α} {i : Nat} {h} : eraseIdx l i = #[] ↔ l.size = 1 ∧ i = 0 := by
   rcases l with ⟨l⟩
   simp only [List.eraseIdx_toArray, mk.injEq, List.eraseIdx_eq_nil_iff, size_toArray,
     or_iff_right_iff_imp]
   rintro rfl
   simp_all
 
-theorem eraseIdx_ne_nil_iff {l : Array α} {i : Nat} {h} : eraseIdx l i ≠ #[] ↔ 2 ≤ l.size := by
+theorem eraseIdx_ne_empty_iff {l : Array α} {i : Nat} {h} : eraseIdx l i ≠ #[] ↔ 2 ≤ l.size := by
   rcases l with ⟨_ | ⟨a, (_ | ⟨b, l⟩)⟩⟩
   · simp
   · simp at h
@@ -319,179 +332,69 @@ theorem mem_of_mem_eraseIdx {l : Array α} {i : Nat} {h} {a : α} (h : a ∈ l.e
   rcases l with ⟨l⟩
   simpa using List.mem_of_mem_eraseIdx (by simpa using h)
 
-@[simp]
-theorem eraseIdx_eq_self : ∀ {l : List α} {k : Nat}, eraseIdx l k = l ↔ length l ≤ k
-  | [], _ => by simp
-  | a::l, 0 => by simp [(cons_ne_self _ _).symm]
-  | a::l, k + 1 => by simp [eraseIdx_eq_self]
-
-theorem eraseIdx_of_length_le {l : List α} {k : Nat} (h : length l ≤ k) : eraseIdx l k = l := by
-  rw [eraseIdx_eq_self.2 h]
-
-theorem length_eraseIdx_le (l : List α) (i : Nat) : length (l.eraseIdx i) ≤ length l :=
-  (eraseIdx_sublist l i).length_le
-
-theorem le_length_eraseIdx (l : List α) (i : Nat) : length l - 1 ≤ length (l.eraseIdx i) := by
-  rw [length_eraseIdx]
-  split <;> simp
-
-theorem eraseIdx_append_of_lt_length {l : List α} {k : Nat} (hk : k < length l) (l' : List α) :
+theorem eraseIdx_append_of_lt_size {l : Array α} {k : Nat} (hk : k < l.size) (l' : Array α) (h) :
     eraseIdx (l ++ l') k = eraseIdx l k ++ l' := by
-  induction l generalizing k with
-  | nil => simp_all
-  | cons x l ih =>
-    cases k with
-    | zero => rfl
-    | succ k => simp_all [eraseIdx_cons_succ, Nat.succ_lt_succ_iff]
+  rcases l with ⟨l⟩
+  rcases l' with ⟨l'⟩
+  simp at hk
+  simp [List.eraseIdx_append_of_lt_length, *]
 
-theorem eraseIdx_append_of_length_le {l : List α} {k : Nat} (hk : length l ≤ k) (l' : List α) :
-    eraseIdx (l ++ l') k = l ++ eraseIdx l' (k - length l) := by
-  induction l generalizing k with
-  | nil => simp_all
-  | cons x l ih =>
-    cases k with
-    | zero => simp_all
-    | succ k => simp_all [eraseIdx_cons_succ, Nat.succ_sub_succ]
+theorem eraseIdx_append_of_length_le {l : Array α} {k : Nat} (hk : l.size ≤ k) (l' : Array α) (h) :
+    eraseIdx (l ++ l') k = l ++ eraseIdx l' (k - l.size) (by simp at h; omega) := by
+  rcases l with ⟨l⟩
+  rcases l' with ⟨l'⟩
+  simp at hk
+  simp [List.eraseIdx_append_of_length_le, *]
 
-theorem eraseIdx_replicate {n : Nat} {a : α} {k : Nat} :
-    (replicate n a).eraseIdx k = if k < n then replicate (n - 1) a else replicate n a := by
-  split <;> rename_i h
-  · rw [eq_replicate_iff, length_eraseIdx_of_lt (by simpa using h)]
-    simp only [length_replicate, true_and]
-    intro b m
-    replace m := mem_of_mem_eraseIdx m
-    simp only [mem_replicate] at m
-    exact m.2
-  · rw [eraseIdx_of_length_le (by simpa using h)]
+theorem eraseIdx_mkArray {n : Nat} {a : α} {k : Nat} {h} :
+    (mkArray n a).eraseIdx k = mkArray (n - 1) a := by
+  simp at h
+  simp only [← List.toArray_replicate, List.eraseIdx_toArray]
+  simp [List.eraseIdx_replicate, h]
 
-theorem Pairwise.eraseIdx {l : List α} (k) : Pairwise p l → Pairwise p (l.eraseIdx k) :=
-  Pairwise.sublist <| eraseIdx_sublist _ _
+theorem mem_eraseIdx_iff_getElem {x : α} {l} {k} {h} : x ∈ eraseIdx l k h ↔ ∃ i w, i ≠ k ∧ l[i]'w = x := by
+  rcases l with ⟨l⟩
+  simp [List.mem_eraseIdx_iff_getElem, *]
 
-theorem Nodup.eraseIdx {l : List α} (k) : Nodup l → Nodup (l.eraseIdx k) :=
-  Pairwise.eraseIdx k
+theorem mem_eraseIdx_iff_getElem? {x : α} {l} {k} {h} : x ∈ eraseIdx l k h ↔ ∃ i ≠ k, l[i]? = some x := by
+  rcases l with ⟨l⟩
+  simp [List.mem_eraseIdx_iff_getElem?, *]
 
-protected theorem IsPrefix.eraseIdx {l l' : List α} (h : l <+: l') (k : Nat) :
-    eraseIdx l k <+: eraseIdx l' k := by
-  rcases h with ⟨t, rfl⟩
-  if hkl : k < length l then
-    simp [eraseIdx_append_of_lt_length hkl]
-  else
-    rw [Nat.not_lt] at hkl
-    simp [eraseIdx_append_of_length_le hkl, eraseIdx_of_length_le hkl]
-
--- See also `mem_eraseIdx_iff_getElem` and `mem_eraseIdx_iff_getElem?` in
--- `Init/Data/List/Nat/Basic.lean`.
-
-theorem erase_eq_eraseIdx [BEq α] [LawfulBEq α] (l : List α) (a : α) (i : Nat) (w : l.indexOf a = i) :
+theorem erase_eq_eraseIdx_of_idxOf [BEq α] [LawfulBEq α] (l : Array α) (a : α) (i : Nat) (w : l.idxOf a = i) (h : i < l.size) :
     l.erase a = l.eraseIdx i := by
-  subst w
-  rw [erase_eq_iff]
-  by_cases h : a ∈ l
-  · right
-    obtain ⟨as, bs, rfl, h'⟩ := eq_append_cons_of_mem h
-    refine ⟨as, bs, h', by simp, ?_⟩
-    rw [indexOf_append, if_neg h', indexOf_cons_self, eraseIdx_append_of_length_le] <;>
-      simp
-  · left
-    refine ⟨h, ?_⟩
-    rw [eq_comm, eraseIdx_eq_self]
-    exact Nat.le_of_eq (indexOf_eq_length h).symm
+  rcases l with ⟨l⟩
+  simp at w
+  simp [List.erase_eq_eraseIdx_of_idxOf, *]
 
+theorem getElem_eraseIdx_of_lt (l : Array α) (i : Nat) (w : i < l.size) (j : Nat) (h : j < (l.eraseIdx i).size) (h' : j < i) :
+    (l.eraseIdx i)[j] = l[j] := by
+  rcases l with ⟨l⟩
+  simp [List.getElem_eraseIdx_of_lt, *]
 
+theorem getElem_eraseIdx_of_ge (l : Array α) (i : Nat) (w : i < l.size) (j : Nat) (h : j < (l.eraseIdx i).size) (h' : i ≤ j) :
+    (l.eraseIdx i)[j] = l[j + 1]'(by simp at h; omega) := by
+  rcases l with ⟨l⟩
+  simp [List.getElem_eraseIdx_of_ge, *]
 
+theorem eraseIdx_set_eq {l : Array α} {i : Nat} {a : α} {h : i < l.size} :
+    (l.set i a).eraseIdx i (by simp; omega) = l.eraseIdx i := by
+  rcases l with ⟨l⟩
+  simp [List.eraseIdx_set_eq, *]
 
-theorem getElem_eraseIdx_of_lt (l : List α) (i : Nat) (j : Nat) (h : j < (l.eraseIdx i).length) (h' : j < i) :
-    (l.eraseIdx i)[j] = l[j]'(by have := length_eraseIdx_le l i; omega) := by
-  rw [getElem_eraseIdx]
-  simp only [dite_eq_left_iff, Nat.not_lt]
-  intro h'
-  omega
+theorem eraseIdx_set_lt {l : Array α} {i : Nat} {w : i < l.size} {j : Nat} {a : α} (h : j < i) :
+    (l.set i a).eraseIdx j (by simp; omega) = (l.eraseIdx j).set (i - 1) a (by simp; omega) := by
+  rcases l with ⟨l⟩
+  simp [List.eraseIdx_set_lt, *]
 
-theorem getElem_eraseIdx_of_ge (l : List α) (i : Nat) (j : Nat) (h : j < (l.eraseIdx i).length) (h' : i ≤ j) :
-    (l.eraseIdx i)[j] = l[j + 1]'(by rw [length_eraseIdx] at h; split at h <;> omega) := by
-  rw [getElem_eraseIdx, dif_neg]
-  omega
-
-theorem eraseIdx_eq_dropLast (l : List α) (i : Nat) (h : i + 1 = l.length) :
-    l.eraseIdx i = l.dropLast := by
-  simp [eraseIdx_eq_take_drop_succ, h]
-  rw [take_eq_dropLast h]
-
-theorem eraseIdx_set_eq {l : List α} {i : Nat} {a : α} :
-    (l.set i a).eraseIdx i = l.eraseIdx i := by
-  apply ext_getElem
-  · simp [length_eraseIdx]
-  · intro n h₁ h₂
-    rw [getElem_eraseIdx, getElem_eraseIdx]
-    split <;>
-    · rw [getElem_set_ne]
-      omega
-
-theorem eraseIdx_set_lt {l : List α} {i : Nat} {j : Nat} {a : α} (h : j < i) :
-    (l.set i a).eraseIdx j = (l.eraseIdx j).set (i - 1) a := by
-  apply ext_getElem
-  · simp [length_eraseIdx]
-  · intro n h₁ h₂
-    simp only [length_eraseIdx, length_set] at h₁
-    simp only [getElem_eraseIdx, getElem_set]
-    split
-    · split
-      · split
-        · rfl
-        · omega
-      · split
-        · omega
-        · rfl
-    · split
-      · split
-        · rfl
-        · omega
-      · have t : i - 1 ≠ n := by omega
-        simp [t]
-
-theorem eraseIdx_set_gt {l : List α} {i : Nat} {j : Nat} {a : α} (h : i < j) :
-    (l.set i a).eraseIdx j = (l.eraseIdx j).set i a := by
-  apply ext_getElem
-  · simp [length_eraseIdx]
-  · intro n h₁ h₂
-    simp only [length_eraseIdx, length_set] at h₁
-    simp only [getElem_eraseIdx, getElem_set]
-    split
-    · rfl
-    · split
-      · split
-        · rfl
-        · omega
-      · have t : i ≠ n := by omega
-        simp [t]
+theorem eraseIdx_set_gt {l : Array α} {i : Nat} {j : Nat} {a : α} (h : i < j) {w : j < l.size} :
+    (l.set i a).eraseIdx j (by simp; omega) = (l.eraseIdx j).set i a (by simp; omega) := by
+  rcases l with ⟨l⟩
+  simp [List.eraseIdx_set_gt, *]
 
 @[simp] theorem set_getElem_succ_eraseIdx_succ
-    {l : List α} {i : Nat} (h : i + 1 < l.length) :
-    (l.eraseIdx (i + 1)).set i l[i + 1] = l.eraseIdx i := by
-  apply ext_getElem
-  · simp only [length_set, length_eraseIdx, h, ↓reduceIte]
-    rw [if_pos]
-    omega
-  · intro n h₁ h₂
-    simp [getElem_set, getElem_eraseIdx]
-    split
-    · split
-      · omega
-      · simp_all
-    · split
-      · split
-        · rfl
-        · omega
-      · have t : ¬ n < i := by omega
-        simp [t]
+    {l : Array α} {i : Nat} (h : i + 1 < l.size) :
+    (l.eraseIdx (i + 1)).set i l[i + 1] (by simp; omega) = l.eraseIdx i := by
+  rcases l with ⟨l⟩
+  simp [List.set_getElem_succ_eraseIdx_succ, *]
 
-@[simp] theorem eraseIdx_length_sub_one (l : List α) :
-    (l.eraseIdx (l.length - 1)) = l.dropLast := by
-  apply ext_getElem
-  · simp [length_eraseIdx]
-    omega
-  · intro n h₁ h₂
-    rw [getElem_eraseIdx_of_lt, getElem_dropLast]
-    simp_all
-
-end List
+end Array
